WeakOmegaCat/TypeSystem/lib.v
@@ -1,0 +1,146 @@
+(* -*- coq-prog-name: "coqtop"; -*- *)
+
+Require Import Coq.Logic.JMeq.
+Require Import ssreflect ssrfun ssrbool .
+
+Require Import libhomot.
+Set Bullet Behavior "Strict Subproofs".
+Set Implicit Arguments.
+
+Unset Strict Implicit.
+Unset Printing Implicit Defensive.
+
+Notation "x ..1" := (projT1 x) (at level 2).
+Notation "x ..2" := (projT2 x) (at level 2).
+Notation "x ,Σ y" := (existT _ x y)  (at level 70).
+Notation "x ≅ y" := (JMeq  x  y) (at level 70, y at next level, no associativity).
+
+Ltac etrans := eapply trans_eq.
+
+Definition is_center (A : Type) (a : A) :=
+  forall ( a' : A),  a' = a.
+Lemma transport (A : Type) (x : A) (P : A -> Type) (y : A)(e : x = y)  (Px : P x) : P y.
+Proof.
+  apply:eq_rect e => //=.
+Defined.
+Lemma transport2 (A : Type)  (P : A -> Type)(Q : forall (a:A), P a -> Type)
+      (x : A) (p : P x)(y : A)(q : P y)(e : x = y)(e' : p ≅ q)  (Px : Q _ p) : Q _ q.
+Proof.
+  destruct e.
+  apply JMeq_eq in e'.
+  by destruct e'.
+Defined.
+
+(* je le réécris en defined *)
+Lemma JMeq_sym : forall (A B:Type) (x:A) (y:B), JMeq x y -> JMeq y x.
+Proof. 
+intros; destruct H; trivial.
+Defined.
+
+Axiom funext : forall (A : Type) (B : A -> Type) (f g : forall a, B a),
+    (forall a, f a = g a) -> f = g.
+
+Lemma uip (A : Type) (x y : A) (e e' : x =y) : e = e'.
+  apply JMeq_eq.
+  destruct e.
+  destruct e'.
+  reflexivity.
+Qed.
+Lemma JMeq_eq_refl A (x  : A) : JMeq_eq (JMeq_refl (x:=x)) = erefl.
+  apply:uip.
+  Qed.
+Lemma JMeq_eq_rect (A : Type) (x : A) (P : A -> Type) (Px : P x) (y : A) (w : x= y) :
+      eq_rect x P Px y w ≅ Px.
+  now destruct w.
+Defined.
+Lemma JMeq_eq_rect_r (A : Type) (x : A) (P : A -> Type) (Px : P x) (y : A) (w : y= x) :
+      @eq_rect_r A x P Px y w ≅ Px.
+  now destruct w.
+Defined.
+
+Lemma JM_eq_eq_rect_r (A : Type) (x : A) (P : A -> Type) (Px : P x) (y : A) (w : y= x) Py :
+    Px ≅ Py ->
+      @eq_rect_r A x P Px y w = Py.
+  destruct w.
+  now move/(@JMeq_eq _ _ _).
+Qed.
+Lemma JM_eq_eq_rect (A : Type) (x : A) (P : A -> Type) (Px : P x) (y : A) (w : x= y) Py :
+    Px ≅ Py ->
+      @eq_rect A x P Px y w = Py.
+  destruct w.
+  now move/(@JMeq_eq _ _ _).
+Qed.
+
+Lemma JMeq_transport (A : Type) (x : A) (P : A -> Type) (Px : P x) (y : A) (w : x= y) :
+      @transport A x P y w Px ≅ Px.
+  now destruct w.
+Qed.
+Lemma JMeq_transport2  (A : Type)  (P : A -> Type)(Q : forall (a:A), P a -> Type)
+      (x : A) (p : P x)(y : A)(q : P y)(e : x = y)(e' : p ≅ q)  (Px : Q _ p) :
+  transport2 e e' Px ≅ Px.
+Proof.
+  destruct e.
+  simpl.
+  by destruct (JMeq_eq e').
+Qed.
+Lemma JM_projT2  (A : Type) (P : A -> Type) (a b : {x : A & P x})
+      (e : a = b) : a..2 ≅ b..2.
+Proof.
+  now destruct e.
+Qed.
+
+Lemma JMeq_from_eq (A : Type) (x y : A) : x = y -> x ≅ y.
+  by destruct 1.
+Qed.
+
+Ltac clear_jmsigma :=
+  match goal with
+  | x : (?C ,Σ ?D) = (_ ,Σ ?E) |- _ =>
+     (apply JM_projT2,JMeq_eq in x; simpl in x)
+    (* have {x} x : D = E by apply : JMeq_eq;apply:(JM_projT2  x) *)
+  | x : ?C = ?C |- _ => clear x
+  end.
+
+  
+
+Lemma JMeq_eq_r  (A : Type) (x y : A) : x = y -> x ≅ y.
+now destruct 1.
+Qed.
+
+Lemma JMeq_congr3 (A : Type) (B : A -> Type)(D: Type) (C : forall a : A, B a -> D)
+      (x x' : A) (b : B x) (b'  : B x') : x = x' -> b ≅ b' -> C x b = C x' b'.
+destruct 1.
+move => eb.
+apply JMeq_eq in eb.
+now destruct eb.
+Qed.
+Lemma JMeq_congr4 (A : Type) (B : A -> Type) (C : forall a : A, B a -> Type)
+      (D : Type) (E : forall a b (c : @C a b), D)
+      (x x' : A) (b : B x) (b'  : B x')
+      (c : C _ b) (c' : C _ b')
+  : x = x' -> b ≅ b' -> c ≅ c' -> E  _ _ c =  E _ _ c'.
+destruct 1.
+move => eb ec.
+apply JMeq_eq in eb.
+destruct eb.
+apply JMeq_eq in ec.
+now destruct ec.
+Qed.
+Lemma JMeq_reflh_eq_rect_r (A : Type) (x : A) (P : A -> Type) (Px : P x) (y : A) (w : y= x) :
+      reflh (@eq_rect_r A x P Px y w) ≅ reflh Px.
+  now destruct w.
+Qed.
+
+Lemma JMeq_Σ (A : Type) (P : A -> Type) (x x': A) (y : P x) (y' : P x') :
+  x = x' -> y ≅ y' -> x ,Σ y = (x' ,Σ y').
+destruct 1.
+move/(@JMeq_eq _ _ _).
+now destruct 1.
+Qed.
+Lemma JMeq_eqh (A B : Type) (x y : A) (x' y':B) (e : A = B) (ex : x ≅ x')
+      (ey: y ≅ y') : (x =h y) = (x' =h y').
+  destruct e.
+  apply JMeq_eq in ex.
+  apply JMeq_eq in ey.
+  by destruct ex, ey.
+Qed.
